theories/typing/case.v
@@ -8,7 +8,7 @@ Section case.
   Context `{typeG Σ}.
 
   (* FIXME : the doc does not give [p +ₗ #(S (ty.(ty_size))) ◁ ...]. *)
-  Lemma type_case_own E L C T p n tyl el:
+  Lemma type_case_own E L C T p n tyl el :
     Forall2 (λ ty e,
       typed_body E L C ((p +ₗ #0 ◁ own n (uninit 1)) :: (p +ₗ #1 ◁ own n ty) ::
          (p +ₗ #(S (ty.(ty_size))) ◁
@@ -49,7 +49,17 @@ Section case.
       iFrame. iExists i, vl', vl''. rewrite /= app_length nth_lookup EQty. auto.
   Qed.
 
-  Lemma type_case_uniq E L C T p κ tyl el:
+  Lemma type_case_own' E L C T T' p n tyl el :
+    tctx_extract_hasty E L p (own n (sum tyl)) T T' →
+    Forall2 (λ ty e,
+      typed_body E L C ((p +ₗ #0 ◁ own n (uninit 1)) :: (p +ₗ #1 ◁ own n ty) ::
+         (p +ₗ #(S (ty.(ty_size))) ◁
+            own n (uninit (list_max (map ty_size tyl) - ty_size ty))) :: T') e ∨
+      typed_body E L C ((p ◁ own n (sum tyl)) :: T') e) tyl el →
+    typed_body E L C T (case: !p of el).
+  Proof. unfold tctx_extract_hasty. intros ->. apply type_case_own. Qed.
+
+  Lemma type_case_uniq E L C T p κ tyl el :
     lctx_lft_alive E L κ →
     Forall2 (λ ty e,
       typed_body E L C ((p +ₗ #1 ◁ &uniq{κ}ty) :: T) e ∨
@@ -97,6 +107,15 @@ Section case.
       iExists _, _. iFrame. iSplit. done. iSplit; iIntros "!>!#$".
   Qed.
 
+  Lemma type_case_uniq' E L C T T' p κ tyl el :
+    tctx_extract_hasty E L p (&uniq{κ}sum tyl) T T' →
+    lctx_lft_alive E L κ →
+    Forall2 (λ ty e,
+      typed_body E L C ((p +ₗ #1 ◁ &uniq{κ}ty) :: T') e ∨
+      typed_body E L C ((p ◁ &uniq{κ}sum tyl) :: T') e) tyl el →
+    typed_body E L C T (case: !p of el).
+  Proof. unfold tctx_extract_hasty. intros ->. apply type_case_uniq. Qed.
+
   Lemma type_case_shr E L C T p κ tyl el:
     lctx_lft_alive E L κ →
     Forall2 (λ ty e,
@@ -121,5 +140,15 @@ Section case.
       rewrite !tctx_interp_cons !tctx_hasty_val' /= ?Hv //; iFrame "HT".
     - iExists _. auto.
     - iExists _. iSplit. done. iExists i. rewrite nth_lookup EQty /=. auto.
+  Qed.
+
+  Lemma type_case_shr' E L C T p κ tyl el :
+    (p ◁ &shr{κ}sum tyl)%TC ∈ T →
+    lctx_lft_alive E L κ →
+    Forall2 (λ ty e, typed_body E L C ((p +ₗ #1 ◁ &shr{κ}ty) :: T) e) tyl el →
+    typed_body E L C T (case: !p of el).
+  Proof.
+    intros. rewrite ->copy_elem_of_tctx_incl; last done; last apply _.
+    apply type_case_shr; first done. eapply Forall2_impl; first done. auto.
   Qed.
 End case.
